compiler/backend/passes/proofs/env_boxProofScript.sml
@@ -14,19 +14,126 @@ val _ = new_theory "env_boxProof";
 
 val _ = set_grammar_ancestry ["env_box_1Proof","env_box"];
 
+Theorem to_box_compile_rel:
+  (∀x x1 b1.
+     to_box x = (x1,b1) ⇒
+     compile_rel (exp_of x) (exp_of x1) ∧
+     (b1 ⇒ can_box (exp_of x1))) ∧
+  (∀x x1.
+     to_box_letrec x = x1 ⇒
+     LIST_REL (λ(m,x) (n,x1).
+       m = n ∧ compile_rel (exp_of x) (exp_of x1)) x x1) ∧
+  (∀x x1 b1.
+     to_box_list x = (x1,b1) ⇒
+     LIST_REL (λx x1. compile_rel (exp_of x) (exp_of x1)) x x1 ∧
+     (b1 ⇒ EVERY (can_box o exp_of) x1))
+Proof
+  ho_match_mp_tac to_box_ind
+  \\ cheat
+QED
+
 Theorem itree_of_compile_to_box:
   closed (exp_of x) ⇒
   itree_of (exp_of x) =
-  itree_of (exp_of (env_box$compile_to_box c x))
+  itree_of (exp_of (compile_to_box c x))
 Proof
-  cheat
+  rw [compile_to_box_def]
+  \\ pairarg_tac \\ gvs []
+  \\ gvs [itree_of_def]
+  \\ irule compile_rel_semantics \\ fs []
+  \\ imp_res_tac to_box_compile_rel
+QED
+
+Triviality MAP2_NIL:
+  ∀xs ys. LENGTH ys = LENGTH xs ⇒ (MAP2 f xs ys = [] ⇔ xs = [])
+Proof
+  Induct \\ Cases_on ‘ys’ \\ gvs []
 QED
 
 Theorem compile_to_box_wf:
-  cexp_wf (env_box$compile_to_box c x) = cexp_wf x ∧
-  cns_arities (env_box$compile_to_box c x) = cns_arities x
+  cexp_wf (compile_to_box c x) = cexp_wf x ∧
+  cns_arities (compile_to_box c x) = cns_arities x
 Proof
-  cheat
+  simp [compile_to_box_def]
+  \\ IF_CASES_TAC \\ fs []
+  \\ pairarg_tac \\ fs []
+  \\ qsuff_tac ‘
+       (∀x e1 b. to_box x = (e1,b) ⇒
+                 cexp_wf e1 = cexp_wf x ∧
+                 cns_arities e1 = cns_arities x) ∧
+       (∀x e1. to_box_letrec x = e1 ⇒
+               LENGTH e1 = LENGTH x ∧
+               MAP (λ(p1,p2). explode p1) e1 =
+               MAP (λ(p1,p2). explode p1) x ∧
+               EVERY (λ(_,x). ∃n m. x = Lam n m ∨ x = Delay m) e1 =
+               EVERY (λ(_,x). ∃n m. x = Lam n m ∨ x = Delay m) x ∧
+               LIST_REL (λa b. cexp_wf (SND a) = cexp_wf (SND b)) x e1 ∧
+               BIGUNION (set (MAP (λa. cns_arities (SND a)) e1)) =
+               BIGUNION (set (MAP (λa. cns_arities (SND a)) x))) ∧
+       (∀x e1 b. to_box_list x = (e1,b) ⇒
+                 LENGTH e1 = LENGTH x ∧
+                 LIST_REL (λa b. cexp_wf a = cexp_wf b) x e1 ∧
+                 BIGUNION (set (MAP (λa. cns_arities a) e1)) =
+                 BIGUNION (set (MAP (λa. cns_arities a) x)))’
+  >- (rw [] \\ res_tac \\ fs [])
+  \\ rpt $ pop_assum kall_tac
+  \\ ho_match_mp_tac to_box_ind
+  \\ rpt conj_tac
+  \\ rpt (disch_tac ORELSE gen_tac)
+  \\ gvs [to_box_def]
+  \\ rpt (pairarg_tac \\ gvs [])
+  \\ gvs [AllCaseEqs(),cns_arities_def]
+  >- gvs [LIST_REL_EL_EQN,EVERY_EL]
+  >-
+   (‘MAP FST (MAP2 (λ(n,cs,_) e. (n,cs,e)) rs ys) = MAP FST rs ∧
+     MAP (explode ∘ FST) (MAP2 (λ(n,cs,_) e. (n,cs,e)) rs ys) =
+     MAP (explode ∘ FST) rs ∧
+     MAP (λ(cn,vs,e). (explode cn,LENGTH vs))
+              (MAP2 (λ(n,cs,_) e. (n,cs,e)) rs ys) =
+     MAP (λ(cn,vs,e). (explode cn,LENGTH vs)) rs ∧
+     MAP (λ(cn,vs,e). cns_arities e)
+                (MAP2 (λ(n,cs,_) e. (n,cs,e)) rs ys) =
+     MAP (λe. cns_arities e) ys ∧
+     MAP (λ(p1,p1',p2). p1') (MAP2 (λ(n,cs,_) e. (n,cs,e)) rs ys) =
+     MAP (λ(p1,p1',p2). p1') rs’ by
+     (qpat_x_assum ‘LENGTH _ = LENGTH _’ mp_tac
+      \\ qid_spec_tac ‘ys’
+      \\ qid_spec_tac ‘rs’
+      \\ rpt $ pop_assum kall_tac
+      \\ Induct \\ Cases_on ‘ys’ \\ gvs []
+      \\ gvs [FORALL_PROD] \\ rw []) \\ fs []
+    \\ gvs [EVERY_MAP]
+    \\ ‘EVERY (λx. (λ(_,vs,x'). ALL_DISTINCT vs ∧ cexp_wf x') x)
+          (MAP2 (λ(n,cs,_) e. (n,cs,e)) rs ys) =
+        EVERY (λx. (λ(_,vs,x'). ALL_DISTINCT vs ∧ cexp_wf x') x) rs’ by
+     (qpat_x_assum ‘LIST_REL _ _ _’ mp_tac
+      \\ qid_spec_tac ‘ys’
+      \\ qid_spec_tac ‘rs’
+      \\ rpt $ pop_assum kall_tac
+      \\ Induct \\ Cases_on ‘ys’ \\ gvs []
+      \\ gvs [FORALL_PROD] \\ rw [])
+    \\ Cases_on ‘d’ \\ gvs []
+    \\ gvs [MAP_MAP_o,o_DEF,LAMBDA_PROD,MAP2_NIL]
+    \\ PairCases_on ‘x’ \\ gvs []
+    \\ pairarg_tac \\ gvs [])
+  >-
+   (gvs [LAMBDA_PROD,EVERY_MAP]
+    \\ ‘EVERY (λ(p1,p2). cexp_wf p2) (to_box_letrec x) =
+        EVERY (λ(p1,p2). cexp_wf p2) x’ by
+      gvs [LIST_REL_EL_EQN,EVERY_EL,UNCURRY]
+    \\ gvs [])
+  \\ Cases_on ‘dest_Delay x’ \\ gvs []
+  >-
+   (qsuff_tac ‘(∃n m. e1 = Lam n m ∨ e1 = Delay m) =
+               (∃n m. x = Lam n m ∨ x = Delay m)’ >- fs []
+    \\ Cases_on ‘x’ \\ gvs [to_box_def,dest_Delay_def]
+    \\ rpt (pairarg_tac \\ gvs [])
+    \\ Cases_on ‘c’ \\ gvs [to_box_def]
+    \\ rpt (pairarg_tac \\ gvs []))
+  \\ ‘∃y. x = Delay y’ by (Cases_on ‘x’ \\ gvs [dest_Delay_def])
+  \\ gvs [dest_Delay_def]
+  \\ rpt (pairarg_tac \\ gvs [])
+  \\ gvs [cns_arities_def]
 QED
 
 val _ = export_theory ();
